src/SDK/AwsCryptographicMaterialsProviderClient.dfy
@@ -1,0 +1,114 @@
+// Copyright Amazon.com Inc. or its affiliates. All Rights Reserved.
+// SPDX-License-Identifier: Apache-2.0
+
+include "../StandardLibrary/StandardLibrary.dfy"
+include "../StandardLibrary/UInt.dfy"
+include "Materials.dfy"
+include "EncryptionContext.dfy"
+include "CMM/Defs.dfy"
+include "MessageHeader.dfy"
+include "MessageBody.dfy"
+include "Serialize.dfy"
+include "Deserialize.dfy"
+include "Keyring/Defs.dfy"
+include "../Crypto/Random.dfy"
+include "../Util/Streams.dfy"
+include "../Crypto/KeyDerivationAlgorithms.dfy"
+include "../Crypto/HKDF/HKDF.dfy"
+include "../Crypto/AESEncryption.dfy"
+include "../Crypto/Signature.dfy"
+include "../Generated/AwsCryptographicMaterialProviders.dfy"
+include "../Generated/AwsEncryptionSdk.dfy"
+include "../Util/UTF8.dfy"
+include "../Crypto/EncryptionSuites.dfy"
+include "Keyring/PolymorphRawAESKeyring.dfy"
+include "CMM/PolymorphDefaultCMM.dfy"
+include "Client.dfy"
+
+module {:extern "MaterialsProviderClientDefs"} MaterialsProviderClientDefs {
+  import opened Wrappers
+  import opened StandardLibrary
+  import opened UInt = StandardLibrary.UInt
+  import AlgorithmSuite
+  import EncryptionSuites
+  import UTF8
+  import Aws.Crypto
+  import PolymorphDefaultCMMDef
+  import PolymorphRawAESKeyringDef
+  import Aws.Esdk
+  import Client = ESDKClient
+
+  const VALID_ALGORITHMS := {EncryptionSuites.AES_GCM_128, EncryptionSuites.AES_GCM_192, EncryptionSuites.AES_GCM_256}
+
+  class MaterialsProviderClient extends Crypto.IAwsCryptographicMaterialsProviderClient {
+    constructor () {}
+
+    method CreateRawAesKeyring(input: Crypto.CreateRawAesKeyringInput) returns (res: Crypto.IKeyring)
+      requires input.Valid()
+    {
+      var wrappingAlg:EncryptionSuites.EncryptionSuite;
+      if (input.wrappingAlg==Crypto.ALG_AES128_GCM_IV12_TAG16) {
+        wrappingAlg := EncryptionSuites.AES_GCM_128;
+      } else if (input.wrappingAlg==Crypto.ALG_AES192_GCM_IV12_TAG16) {
+        wrappingAlg := EncryptionSuites.AES_GCM_192;
+      } else {
+        assert input.wrappingAlg==Crypto.ALG_AES256_GCM_IV12_TAG16;
+        wrappingAlg := EncryptionSuites.AES_GCM_256;
+      }
+      // I have no idea why :- isn't working here...
+      var namespaceRes := UTF8.Encode(input.keyNamespace);
+      var namespace;
+      if namespaceRes.Success? {
+        namespace := namespaceRes.value;
+      }
+      var nameRes := UTF8.Encode(input.keyName);
+      var name;
+      if nameRes.Success? {
+        name := nameRes.value;
+      }
+      assert wrappingAlg in VALID_ALGORITHMS;
+      assert wrappingAlg.Valid(); 
+
+      expect |namespace| < UINT16_LIMIT;
+      expect |input.wrappingKey| == 16 || |input.wrappingKey| == 24 || |input.wrappingKey| == 32;
+      expect |input.wrappingKey| == wrappingAlg.keyLen as int;
+      
+      return new PolymorphRawAESKeyringDef.PolymorphRawAESKeyring(namespace, name, input.wrappingKey, wrappingAlg);
+    }
+
+    method CreateDefaultCryptographicMaterialsManager(input: Crypto.CreateDefaultCryptographicMaterialsManagerInput) returns (res: Crypto.ICryptographicMaterialsManager)
+      requires input.Valid()
+    {
+        expect input.keyring.Valid();
+        return new PolymorphDefaultCMMDef.PolymorphDefaultCMM.OfKeyring(input.keyring);
+    }
+  }
+
+  // move to different module
+  class PolymorphClient extends Esdk.IAwsEncryptionSdkClient {
+        constructor () {}
+
+        method Encrypt(input: Esdk.EncryptInput) returns (res: Result<Esdk.EncryptOutput, string>)
+            requires input.Valid()
+            ensures input.materialsManager.Valid()
+        {
+            expect input.materialsManager.Valid();
+            var encryptRequest := Client.EncryptRequest.WithCMM(input.plaintext, input.materialsManager).SetEncryptionContext(input.encryptionContext);
+            var e :- expect Client.Encrypt(encryptRequest);
+            // TODO is this weird?
+            expect input.materialsManager.Valid();
+            return Success(Esdk.EncryptOutput(ciphertext:=e));
+        }
+        method Decrypt(input: Esdk.DecryptInput) returns (res: Result<Esdk.DecryptOutput, string>)
+            requires input.Valid()
+            ensures input.materialsManager.Valid()
+        {
+            expect input.materialsManager.Valid();
+            var decryptRequest := Client.DecryptRequest.WithCMM(input.ciphertext, input.materialsManager);
+            var d :- expect Client.Decrypt(decryptRequest);
+            // TODO is this weird?
+            expect input.materialsManager.Valid();
+            return Success(Esdk.DecryptOutput(plaintext:=d));
+        }
+  }
+}
