src/SDK/CMM/PolymorphDefaultCMM.dfy
@@ -1,0 +1,169 @@
+// Copyright Amazon.com Inc. or its affiliates. All Rights Reserved.
+// SPDX-License-Identifier: Apache-2.0
+
+include "../../StandardLibrary/StandardLibrary.dfy"
+include "../../StandardLibrary/UInt.dfy"
+include "../../StandardLibrary/Base64.dfy"
+include "../Materials.dfy"
+include "../EncryptionContext.dfy"
+include "Defs.dfy"
+include "../Keyring/Defs.dfy"
+include "../MessageHeader.dfy"
+include "../../Util/UTF8.dfy"
+include "../Deserialize.dfy"
+include "../../Generated/AwsCryptographicMaterialProviders.dfy"
+
+module {:extern "PolymorphDefaultCMMDef"} PolymorphDefaultCMMDef {
+  import opened Wrappers
+  import opened UInt = StandardLibrary.UInt
+  import Materials
+  import EncryptionContext
+  import CMMDefs
+  import KeyringDefs
+  import AlgorithmSuite
+  import Signature
+  import Base64
+  import MessageHeader
+  import UTF8
+  import Deserialize
+  import Aws.Crypto
+
+  predicate {:opaque } DecryptionMaterialsFromPolymorphDefaultCMM(key: seq<uint8>)
+  {
+    true
+  }
+
+  // TODO move
+  predicate method Serializable(mat:Crypto.EncryptionMaterials) {
+    && |mat.encryptedDataKeys| > 0
+    && EncryptionContext.Serializable(mat.encryptionContext)
+  }
+
+  class PolymorphDefaultCMM extends Crypto.ICryptographicMaterialsManager {
+    const keyring: Crypto.IKeyring
+
+    predicate method Valid()
+      reads this, Repr
+      ensures Valid() ==> this in Repr
+    {
+      this in Repr &&
+      keyring in Repr && keyring.Repr <= Repr && this !in keyring.Repr && keyring.Valid()
+    }
+
+    constructor OfKeyring(k: Crypto.IKeyring)
+      requires k.Valid()
+      ensures keyring == k
+      ensures Valid() && fresh(Repr - k.Repr)
+    {
+      keyring := k;
+      Repr := {this} + k.Repr;
+    }
+
+    method GetEncryptionMaterials(input: Crypto.GetEncryptionMaterialsInput)
+                                  returns (res: Result<Crypto.GetEncryptionMaterialsOutput, string>)
+      requires input.Valid()
+      ensures Valid()
+      // the heck is this?
+      // ensures res.Success? ==> CMMDefs.EncryptionMaterialsSignature(res.value.materials)
+      ensures res.Success? ==> res.value.materials.plaintextDataKey.Some? && Serializable(res.value.materials)
+      ensures Materials.EC_PUBLIC_KEY_FIELD in input.encryptionContext ==> res.Failure?
+      ensures res.Success? && (input.algorithmSuiteID.None? || AlgorithmSuite.PolymorphIDToInternalID(input.algorithmSuiteID.value).SignatureType().Some?) ==>
+        Materials.EC_PUBLIC_KEY_FIELD in res.value.materials.encryptionContext
+      ensures res.Success? ==> Serializable(res.value.materials)
+      ensures res.Success? ==>
+        match input.algorithmSuiteID
+        case Some(id) => res.value.materials.algorithmSuiteID == id
+        case None => AlgorithmSuite.PolymorphIDToInternalID(res.value.materials.algorithmSuiteID) == 0x0378
+    {
+      expect Valid();
+      // reveal CMMDefs.EncryptionMaterialsSignatureOpaque();
+      var reservedField := Materials.EC_PUBLIC_KEY_FIELD;
+      assert reservedField in Materials.RESERVED_KEY_VALUES;
+      if reservedField in input.encryptionContext.Keys {
+        return Failure("Reserved Field found in EncryptionContext keys.");
+      }
+      var id := AlgorithmSuite.AES_256_GCM_IV12_TAG16_HKDF_SHA384_ECDSA_P384;
+      if (input.algorithmSuiteID.Some?) {
+        id := AlgorithmSuite.PolymorphIDToInternalID(input.algorithmSuiteID.value);
+      }
+      var enc_sk := None;
+      var enc_ctx := input.encryptionContext;
+
+      match id.SignatureType() {
+        case None =>
+        case Some(param) =>
+          var signatureKeys :- Signature.KeyGen(param);
+          enc_sk := Some(signatureKeys.signingKey);
+          var enc_vk :- UTF8.Encode(Base64.Encode(signatureKeys.verificationKey));
+          enc_ctx := enc_ctx[reservedField := enc_vk];
+      }
+
+      // Check validity of the encryption context at runtime.
+      var validAAD := EncryptionContext.CheckSerializable(enc_ctx);
+      if !validAAD {
+        //TODO: Provide a more specific error message here, depending on how the EncCtx spec was violated.
+        return Failure("Invalid Encryption Context");
+      }
+      assert EncryptionContext.Serializable(enc_ctx);
+
+      var materials := Crypto.EncryptionMaterials(
+        encryptionContext:=enc_ctx,
+        algorithmSuiteID:=AlgorithmSuite.InternalIDToPolymorphID(id),
+        plaintextDataKey:=None(),
+        encryptedDataKeys:=[],
+        signingKey:=enc_sk
+      );
+      assert materials.encryptionContext == enc_ctx;
+      var result :- keyring.OnEncrypt(Crypto.OnEncryptInput(materials:=materials));
+      if result.materials.plaintextDataKey.None? || |result.materials.encryptedDataKeys| == 0 {
+        return Failure("Could not retrieve materials required for encryption");
+      }
+      assert result.materials.Valid();
+
+      expect result.materials.plaintextDataKey.Some? && Serializable(result.materials);
+      expect (input.algorithmSuiteID.None? || AlgorithmSuite.PolymorphIDToInternalID(input.algorithmSuiteID.value).SignatureType().Some?) ==> Materials.EC_PUBLIC_KEY_FIELD in result.materials.encryptionContext;
+      expect match input.algorithmSuiteID
+        case Some(id) => result.materials.algorithmSuiteID == id
+        case None => AlgorithmSuite.PolymorphIDToInternalID(result.materials.algorithmSuiteID) == 0x0378;
+
+      return Success(Crypto.GetEncryptionMaterialsOutput(materials:=result.materials));
+    }
+
+    method DecryptMaterials(input: Crypto.DecryptMaterialsInput)
+                            returns (res: Result<Crypto.DecryptMaterialsOutput, string>)
+      requires input.Valid()
+      ensures Valid()
+      ensures res.Success? ==> res.value.decryptionMaterials.plaintextDataKey.Some?
+    {
+      expect Valid();
+      // Retrieve and decode verification key from encryption context if using signing algorithm
+      var vkey := None;
+      var algID := AlgorithmSuite.PolymorphIDToInternalID(input.algorithmSuiteID);
+      var encCtx := input.encryptionContext;
+
+      if algID.SignatureType().Some? {
+        var reservedField := Materials.EC_PUBLIC_KEY_FIELD;
+        if reservedField !in encCtx {
+          return Failure("Could not get materials required for decryption.");
+        }
+        var encodedVKey := encCtx[reservedField];
+        var utf8Decoded :- UTF8.Decode(encodedVKey);
+        var base64Decoded :- Base64.Decode(utf8Decoded);
+        vkey := Some(base64Decoded);
+      }
+
+      var materials := Crypto.DecryptionMaterials(
+        encryptionContext:=encCtx,
+        algorithmSuiteID:=input.algorithmSuiteID,
+        plaintextDataKey:=None(),
+        verificationKey:=vkey
+      );
+      var result :- keyring.OnDecrypt(Crypto.OnDecryptInput(materials:=materials, encryptedDataKeys:=input.encryptedDataKeys));
+      if result.materials.plaintextDataKey.None? {
+        return Failure("Keyring.OnDecrypt failed to decrypt the plaintext data key.");
+      }
+
+      return Success(Crypto.DecryptMaterialsOutput(decryptionMaterials:=result.materials));
+    }
+  }
+}
