src/SDK/Keyring/PolymorphRawAESKeyring.dfy
@@ -1,0 +1,405 @@
+// Copyright Amazon.com Inc. or its affiliates. All Rights Reserved.
+// SPDX-License-Identifier: Apache-2.0
+
+include "../../StandardLibrary/StandardLibrary.dfy"
+include "../../StandardLibrary/UInt.dfy"
+include "../AlgorithmSuite.dfy"
+include "./Defs.dfy"
+include "../../Crypto/EncryptionSuites.dfy"
+include "../../Crypto/Random.dfy"
+include "../../Crypto/AESEncryption.dfy"
+include "../Materials.dfy"
+include "../MessageHeader.dfy"
+include "../EncryptionContext.dfy"
+include "../Serialize.dfy"
+include "../../Util/UTF8.dfy"
+include "../../Util/Streams.dfy"
+include "../../Generated/AwsCryptographicMaterialProviders.dfy"
+
+module {:extern "PolymorphRawAESKeyringDef"} PolymorphRawAESKeyringDef {
+  import opened StandardLibrary
+  import opened Wrappers
+  import Aws.Crypto
+  import opened UInt = StandardLibrary.UInt
+  import EncryptionSuites
+  import AlgorithmSuite
+  import Random
+  import KeyringDefs
+  import AESEncryption
+  import Mat = Materials
+  import MessageHeader
+  import UTF8
+  import EncryptionContext
+  import Serialize
+  import Streams
+
+  const AUTH_TAG_LEN_LEN := 4;
+  const IV_LEN_LEN       := 4;
+  const VALID_ALGORITHMS := {EncryptionSuites.AES_GCM_128, EncryptionSuites.AES_GCM_192, EncryptionSuites.AES_GCM_256}
+
+  function method DeserializeEDKCiphertext(ciphertext: seq<uint8>, tagLen: nat): (encOutput: AESEncryption.EncryptionOutput)
+    requires tagLen <= |ciphertext|
+    ensures |encOutput.authTag| == tagLen
+  {
+      var encryptedKeyLength := |ciphertext| - tagLen as int;
+      AESEncryption.EncryptionOutput(ciphertext[.. encryptedKeyLength], ciphertext[encryptedKeyLength ..])
+  }
+
+  function method SerializeEDKCiphertext(encOutput: AESEncryption.EncryptionOutput): (ciphertext: seq<uint8>) {
+    encOutput.cipherText + encOutput.authTag
+  }
+
+  lemma EDKSerializeDeserialize(encOutput: AESEncryption.EncryptionOutput)
+    ensures DeserializeEDKCiphertext(SerializeEDKCiphertext(encOutput), |encOutput.authTag|) == encOutput
+  {}
+
+  lemma EDKDeserializeSerialze(ciphertext: seq<uint8>, tagLen: nat)
+    requires tagLen <= |ciphertext|
+    ensures SerializeEDKCiphertext(DeserializeEDKCiphertext(ciphertext, tagLen)) == ciphertext
+  {}
+
+  class PolymorphRawAESKeyring extends Crypto.IKeyring {
+    const keyNamespace: UTF8.ValidUTF8Bytes
+    const keyName: UTF8.ValidUTF8Bytes
+    const wrappingKey: seq<uint8>
+    const wrappingAlgorithm: EncryptionSuites.EncryptionSuite
+
+    //= compliance/framework/raw-aes-keyring.txt#2.5.1
+    //= type=exception
+    //# The wrapping key MUST be a secret value consisting of
+    //# cryptographically secure pseudo-random bytes.
+
+    //= compliance/framework/raw-aes-keyring.txt#2.5.1
+    //= type=exception
+    //# It MUST be randomly
+    //# generated from a cryptographically secure entropy source.
+
+    predicate method Valid()
+      reads this, Repr
+      ensures Valid() ==> this in Repr
+    {
+      && this in Repr
+      && |wrappingKey| == wrappingAlgorithm.keyLen as int
+      && wrappingAlgorithm in VALID_ALGORITHMS
+      && wrappingAlgorithm.Valid()
+      && |keyNamespace| < UINT16_LIMIT
+    }
+
+    // TODO move to materials
+    predicate method ValidEncryptionMaterials(mat: Crypto.EncryptionMaterials) {
+      && (AlgorithmSuite.PolymorphIDToInternalID(mat.algorithmSuiteID).SignatureType().Some? ==> mat.signingKey.Some?)
+      && (mat.plaintextDataKey.Some? ==> AlgorithmSuite.PolymorphIDToInternalID(mat.algorithmSuiteID).ValidPlaintextDataKey(mat.plaintextDataKey.value))
+      && (mat.plaintextDataKey.None? ==> |mat.encryptedDataKeys| == 0)
+    }
+
+    //= compliance/framework/raw-aes-keyring.txt#2.5
+    //= type=implication
+    //# On keyring initialization, the caller MUST provide the following:
+    constructor (namespace: UTF8.ValidUTF8Bytes, name: UTF8.ValidUTF8Bytes, key: seq<uint8>, wrappingAlg: EncryptionSuites.EncryptionSuite)
+      requires |namespace| < UINT16_LIMIT
+      requires wrappingAlg in VALID_ALGORITHMS
+      requires wrappingAlg.Valid()
+
+      //= compliance/framework/raw-aes-keyring.txt#2.5.1
+      //= type=implication
+      //# The length
+      //# of the wrapping key MUST be 128, 192, or 256.
+      // TODO what does a condition like this mean for the shim?
+      requires |key| == 16 || |key| == 24 || |key| == 32
+      requires |key| == wrappingAlg.keyLen as int
+      ensures keyNamespace == namespace
+      ensures keyName == name
+      ensures wrappingKey == key
+      ensures wrappingAlgorithm == wrappingAlg
+      ensures Valid() && fresh(Repr)
+    {
+      keyNamespace := namespace;
+      keyName := name;
+      wrappingKey := key;
+      wrappingAlgorithm := wrappingAlg;
+      Repr := {this};
+    }
+
+    function method SerializeProviderInfo(iv: seq<uint8>): seq<uint8>
+      requires Valid()
+      requires |iv| == wrappingAlgorithm.ivLen as int
+      reads Repr
+    {
+        keyName +
+        [0, 0, 0, wrappingAlgorithm.tagLen * 8] + // tag length in bits
+        [0, 0, 0, wrappingAlgorithm.ivLen] + // IV length in bytes
+        iv
+    }
+
+    //= compliance/framework/raw-aes-keyring.txt#2.7.1
+    //= type=implication
+    //# OnEncrypt MUST take encryption materials (structures.md#encryption-
+    //# materials) as input.
+    method OnEncrypt(input: Crypto.OnEncryptInput) returns (res: Result<Crypto.OnEncryptOutput, string>)
+
+      // Keyring Trait conditions
+      // requires Valid()
+      ensures res.Success? ==>
+        && input.materials.encryptionContext == res.value.materials.encryptionContext
+        && input.materials.algorithmSuiteID == res.value.materials.algorithmSuiteID
+        && (input.materials.plaintextDataKey.Some? ==> res.value.materials.plaintextDataKey == input.materials.plaintextDataKey)
+        && input.materials.encryptedDataKeys <= res.value.materials.encryptedDataKeys
+        && input.materials.signingKey == res.value.materials.signingKey
+
+      // EDK created using expected AAD
+      ensures res.Success? ==>
+        && var encCtxSerializable := (reveal EncryptionContext.Serializable(); EncryptionContext.Serializable(input.materials.encryptionContext));
+        && |res.value.materials.encryptedDataKeys| == |input.materials.encryptedDataKeys| + 1
+        && encCtxSerializable
+        && wrappingAlgorithm.tagLen as nat <= |res.value.materials.encryptedDataKeys[|input.materials.encryptedDataKeys|].ciphertext|
+        && var encOutput := DeserializeEDKCiphertext(res.value.materials.encryptedDataKeys[|input.materials.encryptedDataKeys|].ciphertext, wrappingAlgorithm.tagLen as nat);
+        && AESEncryption.EncryptionOutputEncryptedWithAAD(encOutput, EncryptionContext.MapToSeq(input.materials.encryptionContext))
+
+      //= compliance/framework/raw-aes-keyring.txt#2.7.1
+      //= type=implication
+      //# Based on the ciphertext output of the AES-GCM decryption, the keyring
+      //# MUST construct an encrypted data key (structures.md#encrypted-data-
+      //# key) with the following specifics:
+      ensures res.Success? ==>
+        && |res.value.materials.encryptedDataKeys| == |input.materials.encryptedDataKeys| + 1
+        // *  The key provider ID (structures.md#key-provider-id) is this
+        // keyring's key namespace (./keyring-interface.md#key-namespace).
+        && res.value.materials.encryptedDataKeys[|input.materials.encryptedDataKeys|].providerID == keyNamespace
+        // *  The key provider information (structures.md#key-provider-
+        //   information) is serialized as the raw AES keyring key provider
+        //   information (Section 2.6.1).
+        && ValidProviderInfo(res.value.materials.encryptedDataKeys[|input.materials.encryptedDataKeys|].providerInfo)
+        // *  The ciphertext (structures.md#ciphertext) is serialized as the raw
+        // AES keyring ciphertext (Section 2.6.2).
+        // TODO ??? strongly tiw output to SerializeEDKCiphertext
+        // TODO seperate these in spec?
+
+      //= compliance/framework/raw-aes-keyring.txt#2.7.1
+      //= type=implication
+      //# If the keyring cannot serialize
+      //# the encryption context, OnEncrypt MUST fail.
+      ensures !EncryptionContext.Serializable(input.materials.encryptionContext) ==> res.Failure?
+    {
+      // TODO missing ValidMaterials checks
+      expect Valid();
+      expect ValidEncryptionMaterials(input.materials);
+      // Check that the encryption context can be serialized correctly
+      reveal EncryptionContext.Serializable();
+      //= compliance/framework/raw-aes-keyring.txt#2.7.1
+      //# The keyring MUST attempt to serialize the encryption materials'
+      //# (structures.md#encryption-materials) encryption context
+      //# (structures.md#encryption-context-1) in the same format as the
+      //# serialization of message header AAD key value pairs (../data-format/
+      //# message-header.md#key-value-pairs).
+      var valid := EncryptionContext.CheckSerializable(input.materials.encryptionContext);
+      if !valid {
+        return Failure("Unable to serialize encryption context");
+      }
+
+      var materialsWithDataKey := input.materials;
+      //= compliance/framework/raw-aes-keyring.txt#2.7.1
+      //# If the encryption materials (structures.md#encryption-materials) do
+      //# not contain a plaintext data key, OnEncrypt MUST generate a random
+      //# plaintext data key and set it on the encryption materials
+      //# (structures.md#encryption-materials).
+      if materialsWithDataKey.plaintextDataKey.None? {
+        var k :- Random.GenerateBytes(AlgorithmSuite.PolymorphIDToInternalID(input.materials.algorithmSuiteID).KeyLength() as int32);
+        materialsWithDataKey := Crypto.EncryptionMaterials(
+          encryptionContext := materialsWithDataKey.encryptionContext,
+          algorithmSuiteID := materialsWithDataKey.algorithmSuiteID,
+          signingKey := materialsWithDataKey.signingKey,
+          plaintextDataKey := Some(k),
+          encryptedDataKeys := []);
+      }
+
+      var iv :- Random.GenerateBytes(wrappingAlgorithm.ivLen as int32);
+      var providerInfo := SerializeProviderInfo(iv);
+
+      var wr := new Streams.ByteWriter();
+      var _ :- Serialize.SerializeKVPairs(wr, input.materials.encryptionContext);
+      var aad := wr.GetDataWritten();
+      assert aad == EncryptionContext.MapToSeq(input.materials.encryptionContext);
+
+      //= compliance/framework/raw-aes-keyring.txt#2.7.1
+      //# The keyring MUST encrypt the plaintext data key in the encryption
+      //# materials (structures.md#encryption-materials) using AES-GCM.
+      var encryptResult :- AESEncryption.AESEncrypt(wrappingAlgorithm, iv, wrappingKey, materialsWithDataKey.plaintextDataKey.value, aad);
+      var encryptedKey := SerializeEDKCiphertext(encryptResult);
+
+      if UINT16_LIMIT <= |providerInfo| {
+        return Failure("Serialized provider info too long.");
+      }
+      if UINT16_LIMIT <= |encryptedKey| {
+        return Failure("Encrypted data key too long.");
+      }
+      var edk:Crypto.ValidEncryptedDataKey := Crypto.EncryptedDataKey(providerID := keyNamespace, providerInfo := providerInfo, ciphertext := encryptedKey);
+
+      //= compliance/framework/raw-aes-keyring.txt#2.7.1
+      //# The keyring MUST append the constructed encrypted data key to the
+      //# encrypted data key list in the encryption materials
+      //# (structures.md#encryption-materials).
+
+      //= compliance/framework/raw-aes-keyring.txt#2.7.1
+      //# OnEncrypt MUST output the modified encryption materials
+      //# (structures.md#encryption-materials).
+      var edks:seq<Crypto.ValidEncryptedDataKey> := materialsWithDataKey.encryptedDataKeys + [edk];
+      var r := Crypto.EncryptionMaterials(
+        encryptionContext := materialsWithDataKey.encryptionContext,
+        algorithmSuiteID := materialsWithDataKey.algorithmSuiteID,
+        signingKey := materialsWithDataKey.signingKey,
+        plaintextDataKey := materialsWithDataKey.plaintextDataKey,
+        encryptedDataKeys := edks);
+      assert materialsWithDataKey.encryptedDataKeys == input.materials.encryptedDataKeys;
+      assert |edks| == |materialsWithDataKey.encryptedDataKeys| + 1;
+      assert r.encryptedDataKeys == edks;
+      assert |r.encryptedDataKeys| == |edks|;
+      assert |r.encryptedDataKeys| >= |input.materials.encryptedDataKeys|;
+      res := Success(Crypto.OnEncryptOutput(materials := r));
+    }
+
+    //= compliance/framework/raw-aes-keyring.txt#2.7.2
+    //= type=implication
+    //# OnDecrypt MUST take decryption input.materials (structures.md#decryption-
+    //# input.materials) and a list of encrypted data keys
+    //# (structures.md#encrypted-data-key) as input.
+    method OnDecrypt(input: Crypto.OnDecryptInput) returns (res: Result<Crypto.OnDecryptOutput, string>)
+      // Keyring Trait conditions
+      // requires Valid()
+      ensures Valid()
+      ensures |input.encryptedDataKeys| == 0 ==> res.Success? && input.materials == res.value.materials
+      ensures input.materials.plaintextDataKey.Some? ==> res.Success? && input.materials == res.value.materials
+      ensures res.Success? ==>
+          && input.materials.encryptionContext == res.value.materials.encryptionContext
+          && input.materials.algorithmSuiteID == res.value.materials.algorithmSuiteID
+          && (input.materials.plaintextDataKey.Some? ==> res.value.materials.plaintextDataKey == input.materials.plaintextDataKey)
+          && res.value.materials.verificationKey == input.materials.verificationKey
+
+      //= compliance/framework/raw-aes-keyring.txt#2.7.2
+      //= type=TODO
+      //# If the decryption input.materials already contain a plaintext data key, the
+      //# keyring MUST fail and MUST NOT modify the decryption input.materials
+      //# (structures.md#decryption-input.materials).
+      // We don't do this. We just pass through...
+
+      // TODO: ensure non-None when input edk list has edk with valid provider info
+
+      // Plaintext decrypted using expected AAD
+      ensures res.Success? && input.materials.plaintextDataKey.None? && res.value.materials.plaintextDataKey.Some? ==>
+        var encCtxSerializable := (reveal EncryptionContext.Serializable(); EncryptionContext.Serializable(input.materials.encryptionContext));
+        && encCtxSerializable
+        && AESEncryption.PlaintextDecryptedWithAAD(res.value.materials.plaintextDataKey.value, EncryptionContext.MapToSeq(input.materials.encryptionContext))
+
+      // If attempts to decrypt an EDK and the input EC cannot be serialized, return a Failure
+      //= compliance/framework/raw-aes-keyring.txt#2.7.2
+      //= type=implication
+      //# If the keyring cannot
+      //# serialize the encryption context, OnDecrypt MUST fail.
+      ensures input.materials.plaintextDataKey.None? && !EncryptionContext.Serializable(input.materials.encryptionContext) && (exists i :: 0 <= i < |input.encryptedDataKeys| && ShouldDecryptEDK(input.encryptedDataKeys[i])) ==> res.Failure?
+    {
+      // TODO missing ValidMaterials checks
+      expect Valid();
+
+      if input.materials.plaintextDataKey.Some? {
+        return Success(Crypto.OnDecryptOutput(materials:=input.materials));
+      }
+      //= compliance/framework/raw-aes-keyring.txt#2.7.2
+      //# The keyring MUST perform the following actions on each encrypted data
+      //# key (structures.md#encrypted-data-key) in the input encrypted data
+      //# key list, serially, until it successfully decrypts one.
+      var i := 0;
+      while i < |input.encryptedDataKeys|
+        invariant forall prevIndex :: 0 <= prevIndex < i ==> prevIndex < |input.encryptedDataKeys| && !(ShouldDecryptEDK(input.encryptedDataKeys[prevIndex]))
+      {
+        if ShouldDecryptEDK(input.encryptedDataKeys[i]) {
+          //= compliance/framework/raw-aes-keyring.txt#2.7.2
+          //# The keyring MUST attempt to serialize the decryption input.materials'
+          //# (structures.md#decryption-input.materials) encryption context
+          //# (structures.md#encryption-context-1) in the same format as the
+          //# serialization of the message header AAD key value pairs (../data-
+          //# format/message-header.md#key-value-pairs).
+          reveal EncryptionContext.Serializable();
+          var valid := EncryptionContext.CheckSerializable(input.materials.encryptionContext);
+          if !valid {
+            return Failure("Unable to serialize encryption context");
+          }
+          var wr := new Streams.ByteWriter();
+          var _ :- Serialize.SerializeKVPairs(wr, input.materials.encryptionContext);
+
+          //= compliance/framework/raw-aes-keyring.txt#2.7.2
+          //# For each encrypted data key (structures.md#encrypted-data-key), the
+          //# keyring MUST first attempt to deserialize the serialized ciphertext
+          //# (Section 2.6.2) to obtain the encrypted key (Section 2.6.2.1) and
+          //# authentication tag (Section 2.6.2.2), and deserialize the serialized
+          //# key provider info (Section 2.6.1) to obtain the key name (./keyring-
+          //# interface.md#key-name), Section 2.6.1.4, IV length (Section 2.6.1.3),
+          //# and authentication tag length (Section 2.6.1.2).
+          // TODO without mocking there isn't a good way to test this...
+          var aad := wr.GetDataWritten();
+          assert aad == EncryptionContext.MapToSeq(input.materials.encryptionContext);
+          var iv := GetIvFromProvInfo(input.encryptedDataKeys[i].providerInfo);
+          var encryptionOutput := DeserializeEDKCiphertext(input.encryptedDataKeys[i].ciphertext, wrappingAlgorithm.tagLen as nat);
+
+          //= compliance/framework/raw-aes-keyring.txt#2.7.2
+          //# If decrypting, the keyring MUST use AES-GCM with the following
+          //# specifics:
+          // TODO break up in spec
+          var ptKey :- AESEncryption.AESDecrypt(wrappingAlgorithm, wrappingKey, encryptionOutput.cipherText, encryptionOutput.authTag, iv, aad);
+
+          //= compliance/framework/raw-aes-keyring.txt#2.7.2
+          //# If a decryption succeeds, this keyring MUST add the resulting
+          //# plaintext data key to the decryption input.materials and return the
+          //# modified input.materials.
+          if AlgorithmSuite.PolymorphIDToInternalID(input.materials.algorithmSuiteID).ValidPlaintextDataKey(ptKey) { // check for correct key length
+            var r := Crypto.DecryptionMaterials(
+            encryptionContext := input.materials.encryptionContext,
+            algorithmSuiteID := input.materials.algorithmSuiteID,
+            verificationKey := input.materials.verificationKey,
+            plaintextDataKey := Some(ptKey));
+            return Success(Crypto.OnDecryptOutput(materials:=r));
+          } else {
+            // TODO will this ever happen?
+            return Failure("Decryption failed: bad datakey length.");
+          }
+        }
+        i := i + 1;
+      }
+      //= compliance/framework/raw-aes-keyring.txt#2.7.2
+      //= type=TODO
+      //# If no decryption succeeds, the keyring MUST fail and MUST NOT modify
+      //# the decryption materials (structures.md#decryption-materials).
+      // Right now we do the opposite, we always "succeed" does the spec need to change? How does this interoperate?
+      return Success(Crypto.OnDecryptOutput(materials:=input.materials));
+    }
+
+    //= compliance/framework/raw-aes-keyring.txt#2.7.2
+    //# The keyring MUST attempt to decrypt the encrypted data key if and
+    //# only if the following is true:
+    // TODO break up
+    predicate method ShouldDecryptEDK(edk: Crypto.EncryptedDataKey) {
+      edk.providerID == keyNamespace && ValidProviderInfo(edk.providerInfo) && wrappingAlgorithm.tagLen as int <= |edk.ciphertext|
+    }
+
+    // TODO #68: prove providerInfo serializes/deserializes correctly
+    predicate method ValidProviderInfo(info: seq<uint8>)
+    {
+      |info| == |keyName| + AUTH_TAG_LEN_LEN + IV_LEN_LEN + wrappingAlgorithm.ivLen as int &&
+      info[0..|keyName|] == keyName &&
+      //= compliance/framework/raw-aes-keyring.txt#2.6.1.2
+      //= type=implication
+      //# This value MUST be 128.
+      SeqToUInt32(info[|keyName|..|keyName| + AUTH_TAG_LEN_LEN]) == 128 &&
+      SeqToUInt32(info[|keyName|..|keyName| + AUTH_TAG_LEN_LEN]) == wrappingAlgorithm.tagLen as uint32 * 8 &&
+      SeqToUInt32(info[|keyName| + AUTH_TAG_LEN_LEN .. |keyName| + AUTH_TAG_LEN_LEN + IV_LEN_LEN]) == wrappingAlgorithm.ivLen as uint32 &&
+      //= compliance/framework/raw-aes-keyring.txt#2.6.1.3
+      //= type=implication
+      //# This value MUST be 12.
+      SeqToUInt32(info[|keyName| + AUTH_TAG_LEN_LEN .. |keyName| + AUTH_TAG_LEN_LEN + IV_LEN_LEN]) == 12
+    }
+
+    function method GetIvFromProvInfo(info: seq<uint8>): seq<uint8>
+      requires ValidProviderInfo(info)
+    {
+      info[|keyName| + AUTH_TAG_LEN_LEN + IV_LEN_LEN ..]
+    }
+  }
+}
