test/SDK/Keyring/PolymorphRawAESKeyring.dfy
@@ -1,0 +1,284 @@
+// Copyright Amazon.com Inc. or its affiliates. All Rights Reserved.
+// SPDX-License-Identifier: Apache-2.0
+
+include "../../../src/SDK/Keyring/PolymorphRawAESKeyring.dfy"
+include "../../../src/SDK/AlgorithmSuite.dfy"
+include "../../../src/SDK/MessageHeader.dfy"
+include "../../../src/SDK/Materials.dfy"
+include "../../../src/SDK/EncryptionContext.dfy"
+include "../../../src/Crypto/EncryptionSuites.dfy"
+include "../../../src/Crypto/AESEncryption.dfy"
+include "../../../src/StandardLibrary/StandardLibrary.dfy"
+include "../../../src/StandardLibrary/UInt.dfy"
+include "../../../src/Util/UTF8.dfy"
+include "../../../src/Generated/AwsCryptographicMaterialProviders.dfy"
+include "../../Util/TestUtils.dfy"
+
+module TestPolymorphAESKeyring {
+  import opened Wrappers
+  import opened UInt = StandardLibrary.UInt
+  import AESEncryption
+  import PolymorphRawAESKeyringDef
+  import MessageHeader
+  import Materials
+  import EncryptionContext
+  import EncryptionSuites
+  import AlgorithmSuite
+  import UTF8
+  import Aws.Crypto
+  import opened TestUtils
+
+  method {:test} TestOnEncryptOnDecryptGenerateDataKey()
+  {
+    var namespace, name := TestUtils.NamespaceAndName(0);
+    var rawAESKeyring := new PolymorphRawAESKeyringDef.PolymorphRawAESKeyring(namespace, name, seq(32, i => 0), EncryptionSuites.AES_GCM_256);
+    var encryptionContext := TestUtils.SmallEncryptionContext(TestUtils.SmallEncryptionContextVariation.A);
+    ExpectSerializableEncryptionContext(encryptionContext);
+
+    var wrappingAlgorithmID := Crypto.ALG_AES_256_GCM_IV12_TAG16_HKDF_SHA384_ECDSA_P384;
+    var signingKey := seq(32, i => 0);
+    var encryptionMaterialsIn := Crypto.EncryptionMaterials(
+      encryptionContext:=encryptionContext,
+      algorithmSuiteID:=wrappingAlgorithmID,
+      plaintextDataKey:=None(),
+      encryptedDataKeys:=[],
+      signingKey:=Some(signingKey)
+    );
+    var encryptionMaterialsOut :- expect rawAESKeyring.OnEncrypt(Crypto.OnEncryptInput(materials:=encryptionMaterialsIn));
+
+    //= compliance/framework/raw-aes-keyring.txt#2.7.1
+    //= type=test
+    //# The keyring MUST append the constructed encrypted data key to the
+    //# encrypted data key list in the encryption materials
+    //# (structures.md#encryption-materials).
+
+    //= compliance/framework/raw-aes-keyring.txt#2.7.1
+    //= type=test
+    //# OnEncrypt MUST output the modified encryption materials
+    //# (structures.md#encryption-materials).
+    expect |encryptionMaterialsOut.materials.encryptedDataKeys| == 1;
+
+    var pdk := encryptionMaterialsOut.materials.plaintextDataKey;
+    var edk := encryptionMaterialsOut.materials.encryptedDataKeys[0];
+    var verificationKey := seq(32, i => 0);
+
+    var decryptionMaterialsIn := Crypto.DecryptionMaterials(
+      encryptionContext:=encryptionContext,
+      algorithmSuiteID:=wrappingAlgorithmID,
+      plaintextDataKey:=None(),
+      verificationKey:=Some(verificationKey)
+    );
+    var decryptionMaterialsOut :- expect rawAESKeyring.OnDecrypt(Crypto.OnDecryptInput(materials:=decryptionMaterialsIn, encryptedDataKeys:=[edk]));
+
+    //= compliance/framework/raw-aes-keyring.txt#2.7.2
+    //= type=test
+    //# If a decryption succeeds, this keyring MUST add the resulting
+    //# plaintext data key to the decryption materials and return the
+    //# modified materials.
+    expect encryptionMaterialsOut.materials.plaintextDataKey == pdk;
+  }
+
+  method {:test} TestOnEncryptOnDecryptSuppliedDataKey()
+  {
+    var namespace, name := TestUtils.NamespaceAndName(0);
+    var rawAESKeyring := new PolymorphRawAESKeyringDef.PolymorphRawAESKeyring(namespace, name, seq(32, i => 0), EncryptionSuites.AES_GCM_256);
+    var encryptionContext := TestUtils.SmallEncryptionContext(TestUtils.SmallEncryptionContextVariation.A);
+    ExpectSerializableEncryptionContext(encryptionContext);
+
+    var pdk := seq(32, i => 0);
+
+    var wrappingAlgorithmID := Crypto.ALG_AES_256_GCM_IV12_TAG16_HKDF_SHA384_ECDSA_P384;
+    var signingKey := seq(32, i => 0);
+    var encryptionMaterialsIn := Crypto.EncryptionMaterials(
+      encryptionContext:=encryptionContext,
+      algorithmSuiteID:=wrappingAlgorithmID,
+      plaintextDataKey:=Some(pdk),
+      encryptedDataKeys:=[],
+      signingKey:=Some(signingKey)
+    );
+    var encryptionMaterialsOut :- expect rawAESKeyring.OnEncrypt(Crypto.OnEncryptInput(materials:=encryptionMaterialsIn));
+    expect |encryptionMaterialsOut.materials.encryptedDataKeys| == 1;
+
+    var edk := encryptionMaterialsOut.materials.encryptedDataKeys[0];
+    var verificationKey := seq(32, i => 0);
+
+    var decryptionMaterialsIn := Crypto.DecryptionMaterials(
+      encryptionContext:=encryptionContext,
+      algorithmSuiteID:=wrappingAlgorithmID,
+      plaintextDataKey:=None(),
+      verificationKey:=Some(verificationKey)
+    );
+    var decryptionMaterialsOut :- expect rawAESKeyring.OnDecrypt(Crypto.OnDecryptInput(materials:=decryptionMaterialsIn, encryptedDataKeys:=[edk]));
+
+    //= compliance/framework/raw-aes-keyring.txt#2.7.1
+    //= type=test
+    //# The keyring MUST encrypt the plaintext data key in the encryption
+    //# materials (structures.md#encryption-materials) using AES-GCM.
+    // We demonstrate this by showing OnEncrypt then OnDecrypt gets us the same pdk back.
+    expect decryptionMaterialsOut.materials.plaintextDataKey == Some(pdk);
+  }
+
+    method {:test} TestOnDecryptKeyNameMismatch()
+  {
+    var namespace, name := TestUtils.NamespaceAndName(0);
+    var rawAESKeyring := new PolymorphRawAESKeyringDef.PolymorphRawAESKeyring(namespace, name, seq(32, i => 0), EncryptionSuites.AES_GCM_256);
+
+    var mismatchName :- expect UTF8.Encode("mismatched");
+    var mismatchedAESKeyring := new PolymorphRawAESKeyringDef.PolymorphRawAESKeyring(namespace, mismatchName, seq(32, i => 0), EncryptionSuites.AES_GCM_256);
+
+    var encryptionContext := TestUtils.SmallEncryptionContext(TestUtils.SmallEncryptionContextVariation.A);
+    ExpectSerializableEncryptionContext(encryptionContext);
+
+    var pdk := seq(32, i => 0);
+
+    var wrappingAlgorithmID := Crypto.ALG_AES_256_GCM_IV12_TAG16_HKDF_SHA384_ECDSA_P384;
+    var signingKey := seq(32, i => 0);
+    var encryptionMaterialsIn := Crypto.EncryptionMaterials(
+      encryptionContext:=encryptionContext,
+      algorithmSuiteID:=wrappingAlgorithmID,
+      plaintextDataKey:=Some(pdk),
+      encryptedDataKeys:=[],
+      signingKey:=Some(signingKey)
+    );
+    var encryptionMaterialsOut :- expect mismatchedAESKeyring.OnEncrypt(Crypto.OnEncryptInput(materials:=encryptionMaterialsIn));
+    expect |encryptionMaterialsOut.materials.encryptedDataKeys| == 1;
+
+    var edk := encryptionMaterialsOut.materials.encryptedDataKeys[0];
+    var verificationKey := seq(32, i => 0);
+
+    var decryptionMaterialsIn := Crypto.DecryptionMaterials(
+      encryptionContext:=encryptionContext,
+      algorithmSuiteID:=wrappingAlgorithmID,
+      plaintextDataKey:=None(),
+      verificationKey:=Some(verificationKey)
+    );
+    var decryptionMaterialsOut :- expect rawAESKeyring.OnDecrypt(Crypto.OnDecryptInput(materials:=decryptionMaterialsIn, encryptedDataKeys:=[edk]));
+    expect decryptionMaterialsOut.materials.plaintextDataKey.None?;
+  }
+
+  // TODO test for multiple EDKS for OnDecrypt
+  // TODO possibly test failure for one?
+  // or is it easier to verify this...
+
+  // TODO test with EDK that shouldn't be decrypted, so with another Keyring e.g.
+
+  //= compliance/framework/raw-aes-keyring.txt#2.7.1
+  //= type=test
+  //# If the encryption materials (structures.md#encryption-materials) do
+  //# not contain a plaintext data key, OnEncrypt MUST generate a random
+  //# plaintext data key and set it on the encryption materials
+  //# (structures.md#encryption-materials).
+  method {:test} TestOnDecryptNoEDKs()
+  {
+    var namespace, name := TestUtils.NamespaceAndName(0);
+    var rawAESKeyring := new PolymorphRawAESKeyringDef.PolymorphRawAESKeyring(namespace, name, seq(32, i => 0), EncryptionSuites.AES_GCM_256);
+    var wrappingAlgorithmID := Crypto.ALG_AES_256_GCM_IV12_TAG16_HKDF_SHA384_ECDSA_P384;
+    var encryptionContext := TestUtils.SmallEncryptionContext(TestUtils.SmallEncryptionContextVariation.A);
+    var verificationKey := seq(32, i => 0);
+    var decryptionMaterialsIn := Crypto.DecryptionMaterials(
+      encryptionContext:=encryptionContext,
+      algorithmSuiteID:=wrappingAlgorithmID,
+      plaintextDataKey:=None(),
+      verificationKey:=Some(verificationKey)
+    );
+    var decryptionMaterialsOut :- expect rawAESKeyring.OnDecrypt(Crypto.OnDecryptInput(materials:=decryptionMaterialsIn, encryptedDataKeys:=[]));
+    expect decryptionMaterialsOut.materials.plaintextDataKey.None?;
+  }
+
+  //= compliance/framework/raw-aes-keyring.txt#2.7.1
+  //= type=test
+  //# The keyring MUST attempt to serialize the encryption materials'
+  //# (structures.md#encryption-materials) encryption context
+  //# (structures.md#encryption-context-1) in the same format as the
+  //# serialization of message header AAD key value pairs (../data-format/
+  //# message-header.md#key-value-pairs).
+
+  method {:test} TestOnEncryptUnserializableEC()
+  {
+    var namespace, name := TestUtils.NamespaceAndName(0);
+    var rawAESKeyring := new PolymorphRawAESKeyringDef.PolymorphRawAESKeyring(namespace, name, seq(32, i => 0), EncryptionSuites.AES_GCM_256);
+    var unserializableEncryptionContext := generateUnserializableEncryptionContext();
+    ExpectNonSerializableEncryptionContext(unserializableEncryptionContext);
+
+    var wrappingAlgorithmID := Crypto.ALG_AES_256_GCM_IV12_TAG16_HKDF_SHA384_ECDSA_P384;
+    var signingKey := seq(32, i => 0);
+        var encryptionMaterialsIn := Crypto.EncryptionMaterials(
+      encryptionContext:=unserializableEncryptionContext,
+      algorithmSuiteID:=wrappingAlgorithmID,
+      plaintextDataKey:=None(),
+      encryptedDataKeys:=[],
+      signingKey:=Some(signingKey)
+    );
+    var encryptionMaterialsOut := rawAESKeyring.OnEncrypt(Crypto.OnEncryptInput(materials:=encryptionMaterialsIn));
+    expect encryptionMaterialsOut.Failure?;
+  }
+
+  //= compliance/framework/raw-aes-keyring.txt#2.7.2
+  //= type=test
+  //# The keyring MUST attempt to serialize the decryption materials'
+  //# (structures.md#decryption-materials) encryption context
+  //# (structures.md#encryption-context-1) in the same format as the
+  //# serialization of the message header AAD key value pairs (../data-
+  //# format/message-header.md#key-value-pairs).
+  method {:test} TestOnDecryptUnserializableEC()
+  {
+    // Set up valid EDK for decryption
+    var encryptionContext := TestUtils.SmallEncryptionContext(TestUtils.SmallEncryptionContextVariation.A);
+    var namespace, name := TestUtils.NamespaceAndName(0);
+    var rawAESKeyring := new PolymorphRawAESKeyringDef.PolymorphRawAESKeyring(namespace, name, seq(32, i => 0), EncryptionSuites.AES_GCM_256);
+    var wrappingAlgorithmID := Crypto.ALG_AES_256_GCM_IV12_TAG16_HKDF_SHA384_ECDSA_P384;
+    var signingKey := seq(32, i => 0);
+    var encryptionMaterialsIn := Crypto.EncryptionMaterials(
+      encryptionContext:=encryptionContext,
+      algorithmSuiteID:=wrappingAlgorithmID,
+      plaintextDataKey:=None(),
+      encryptedDataKeys:=[],
+      signingKey:=Some(signingKey)
+    );
+    var encryptionMaterialsOut :- expect rawAESKeyring.OnEncrypt(Crypto.OnEncryptInput(materials:=encryptionMaterialsIn));
+    expect encryptionMaterialsOut.materials.plaintextDataKey.Some?;
+    expect |encryptionMaterialsOut.materials.encryptedDataKeys| == 1;
+    var edk := encryptionMaterialsOut.materials.encryptedDataKeys[0];
+
+    // Set up EC that can't be serialized
+    var unserializableEncryptionContext := generateUnserializableEncryptionContext();
+    ExpectNonSerializableEncryptionContext(unserializableEncryptionContext);
+    var verificationKey := seq(32, i => 0);
+
+    var decryptionMaterialsIn := Crypto.DecryptionMaterials(
+      encryptionContext:=unserializableEncryptionContext,
+      algorithmSuiteID:=wrappingAlgorithmID,
+      plaintextDataKey:=None(),
+      verificationKey:=Some(verificationKey)
+    );
+    var decryptionMaterialsOut := rawAESKeyring.OnDecrypt(Crypto.OnDecryptInput(materials:=decryptionMaterialsIn, encryptedDataKeys:=[edk]));
+    expect decryptionMaterialsOut.Failure?;
+  }
+
+  method {:test} TestDeserializeEDKCiphertext() {
+    var ciphertext := [0, 1, 2, 3];
+    var authTag := [4, 5, 6, 7];
+    var serializedEDKCiphertext := ciphertext + authTag;
+    var encOutput := PolymorphRawAESKeyringDef.DeserializeEDKCiphertext(serializedEDKCiphertext, |authTag|);
+
+    expect encOutput.cipherText == ciphertext;
+    expect encOutput.authTag == authTag;
+  }
+
+  method {:test} TestSerializeEDKCiphertext() {
+    var ciphertext := [0, 1, 2, 3];
+    var authTag := [4, 5, 6, 7];
+    var encOutput := AESEncryption.EncryptionOutput(ciphertext, authTag);
+    var serializedEDKCiphertext := PolymorphRawAESKeyringDef.SerializeEDKCiphertext(encOutput);
+
+    expect serializedEDKCiphertext == ciphertext + authTag;
+  }
+
+  method generateUnserializableEncryptionContext() returns (encCtx: EncryptionContext.Map)
+  {
+    var keyA :- expect UTF8.Encode("keyA");
+    var invalidVal := seq(0x1_0000, _ => 0);
+    AssumeLongSeqIsValidUTF8(invalidVal);
+    return map[keyA:=invalidVal];
+  }
+}
